FYP/ShortestPath/Lemmas.lean
@@ -17,7 +17,7 @@ lemma fwStep_le_via_k {n : ℕ} (d : Fin n → Fin n → ℕ∞) (k i j : Fin n)
 --   ∀ i j, fwStep d k i j ≤ d i j := by
 --   sorry
 
-lemma foldl_fwStep_le {n : ℕ} (l : List (Fin n)) : --(d : Fin n → Fin n → ℕ∞) :
+lemma foldl_fwStep_le {n : ℕ} (l : List (Fin n)) :
   ∀ d i j, (l.foldl fwStep d) i j ≤ d i j := by
   induction l with
   | nil =>
@@ -29,6 +29,29 @@ lemma foldl_fwStep_le {n : ℕ} (l : List (Fin n)) : --(d : Fin n → Fin n → 
     have h1 := ih (fwStep d k) i j
     have h2 := fwStep_le_self d k i j
     exact le_trans h1 h2
+
+lemma pathWeight_concat {n : ℕ} (G : Graph n) (p q : Path n) :
+  pathWeight G (concatPath p q)
+    = pathWeight G p + pathWeight G q := by
+    induction p with
+    | nil =>
+      simp [concatPath, pathWeight]
+    | cons u ps ih =>
+      cases ps with
+      | nil =>
+        cases q with
+        | nil =>
+          simp [concatPath, pathWeight]
+        | cons v qs =>
+          -- simp [concatPath, pathWeight]
+          sorry
+      | cons v ps' =>
+        cases q with
+        | nil =>
+          simp [concatPath, pathWeight]
+        | cons w qs =>
+          -- simp [concatPath, pathWeight, ih]
+          sorry
 
 
 end FYP
